lib/pulse/lib/Pulse.Lib.SpinLock.fst
@@ -24,16 +24,26 @@ module U32 = FStar.UInt32
 module B = Pulse.Lib.Box
 module GR = Pulse.Lib.GhostReference
 module CInv = Pulse.Lib.CancellableInvariant
+  
+instance assume_box_is_atomic (r: B.box U32.t) i :
+    is_sync (pts_to r #1.0R i) =
+  admit ()
 
-let lock_inv_aux (r:B.box U32.t) (gr:GR.ref U32.t) (v:slprop) : slprop  =
+let lock_inv_aux l' (r:B.box U32.t) (gr:GR.ref U32.t) (v:slprop) : slprop  =
   exists* i p. pts_to r #1.0R i **
                pts_to gr #p i **
-               (if i = 0ul then v else emp) **
+               on (process_of l') (if i = 0ul then v else emp) **
                pure ((i == 0ul ==> p == 1.0R) /\
                      (i =!= 0ul ==> p == 0.5R)) 
 
-let lock_inv (r:B.box U32.t) (gr:GR.ref U32.t) (v:slprop) : slprop =
-  lock_inv_aux r gr v
+let is_send_if (i: U32.t) (v: slprop) (inst: is_send v) : is_send (if i = 0ul then v else emp) =
+  if i = 0ul then inst else is_send_placeless emp #placeless_emp
+
+instance is_sync_lock_inv_aux l' r gr v : is_sync (lock_inv_aux l' r gr v) =
+  Tactics.Typeclasses.solve
+
+let lock_inv l' (r:B.box U32.t) (gr:GR.ref U32.t) (v:slprop) : slprop =
+  on l' <| lock_inv_aux l' r gr v
 
 [@@CAbstractStruct]
 noeq
@@ -43,32 +53,40 @@ type lock = {
   i : cinv;
 }
 
+let is_send_tag v (inst: is_send v) = emp
+
 let lock_alive l #p v =
-  inv (iname_of l.i) (cinv_vp l.i (lock_inv l.r l.gr v)) ** active l.i p
+  exists* l' inst. in_same_process l' ** is_send_tag v inst **
+  inv (iname_of l.i) (cinv_vp l.i (lock_inv l' l.r l.gr v)) ** active l.i p
+
+instance is_sync_lock_alive = Tactics.Typeclasses.solve
 
 let lock_acquired l = pts_to l.gr #0.5R 1ul
 
 
-fn new_lock (v:slprop)
+fn new_lock (v:slprop) {| inst: is_send v |}
   requires v
   returns l:lock
   ensures lock_alive l v
 {
-  let r = B.alloc 0ul;
   let gr = GR.alloc 0ul;
   rewrite v as (if 0ul = 0ul then v else emp);
-  fold (lock_inv_aux r gr v);
-  fold (lock_inv r gr v);
-  let i = new_cancellable_invariant (lock_inv r gr v);
+  loc_get (); with l'. assert loc l';
+  let r = B.alloc 0ul;
+  unsafe_attest_released v #_ #l';
+  fold (lock_inv_aux l' r gr v);
+  on_intro (lock_inv_aux l' r gr v);
+  fold (lock_inv l' r gr v);
+  let i = new_cancellable_invariant (lock_inv l' r gr v) #_;
   let l = { r; gr; i };
   rewrite each r as l.r;
   rewrite each gr as l.gr;
   rewrite each i as l.i;
+  fold in_same_process l';
+  fold is_send_tag v inst;
   fold (lock_alive l #1.0R v);
   l
 }
-
-
 
 fn rec acquire (#v:slprop) (#p:perm) (l:lock)
   preserves lock_alive l #p v
@@ -76,50 +94,60 @@ fn rec acquire (#v:slprop) (#p:perm) (l:lock)
 {
   unfold (lock_alive l #p v);
   later_credit_buy 1;
+  with l'. assert in_same_process l';
+  unfold in_same_process l'; with l0. assert loc l0; loc_dup l0; fold in_same_process l';
+  with inst. assert is_send_tag v inst;
   let b =
     with_invariants (CInv.iname_of l.i)
       returns b:bool
-      ensures later (cinv_vp l.i (lock_inv l.r l.gr v)) **
+      ensures later (cinv_vp l.i (lock_inv l' l.r l.gr v)) **
               active l.i p **
+              in_same_process l' ** loc l0 ** is_send_tag v inst **
               (if b then v ** pts_to l.gr #0.5R 1ul else emp) {
       later_elim _;
       unpack_cinv_vp l.i;
       unfold lock_inv;
+      is_sync_elim_on (lock_inv_aux l' l.r l.gr v) #_;
       unfold lock_inv_aux;
       with i. assert (pts_to l.r i);
       let b = cas_box l.r 0ul 1ul;
       if b {
+        unsafe_attest_acquired (if i = 0ul then v else emp) #(is_send_if i v inst) #l0;
         elim_cond_true _ _ _;
         rewrite each i as 0ul;
         GR.(l.gr := 1ul);
         GR.share l.gr;
-        fold (lock_inv_aux l.r l.gr v);
-        fold (lock_inv l.r l.gr v);
+        on_intro emp; placeless_emp _ (process_of l');
+        fold (lock_inv_aux l' l.r l.gr v);
+        is_sync_intro_on (lock_inv_aux l' l.r l.gr v) _;
+        fold (lock_inv l' l.r l.gr v);
         pack_cinv_vp l.i;
-        assert (cinv_vp l.i (lock_inv l.r l.gr v) **
+        assert (cinv_vp l.i (lock_inv l' l.r l.gr v) **
                 active l.i p **
                 pts_to l.gr #0.5R 1ul **
                 v);
         let b = true;
         rewrite (v ** pts_to l.gr #0.5R 1ul)
              as (if b then v ** pts_to l.gr #0.5R 1ul else emp);
-        later_intro (CInv.cinv_vp l.i (lock_inv l.r l.gr v));
+        later_intro (CInv.cinv_vp l.i (lock_inv l' l.r l.gr v));
         b
       } else {
         elim_cond_false _ _ _;
-        fold (lock_inv_aux l.r l.gr v);
-        fold (lock_inv l.r l.gr v);
+        fold (lock_inv_aux l' l.r l.gr v);
+        is_sync_intro_on (lock_inv_aux l' l.r l.gr v) _;
+        fold (lock_inv l' l.r l.gr v);
         pack_cinv_vp l.i;
-        assert (cinv_vp l.i (lock_inv l.r l.gr v) **
+        assert (cinv_vp l.i (lock_inv l' l.r l.gr v) **
                 active l.i p);
         let b = false;
         rewrite emp as
                 (if b then v ** pts_to l.gr #0.5R 1ul else emp);
-        later_intro (CInv.cinv_vp l.i (lock_inv l.r l.gr v));
+        later_intro (CInv.cinv_vp l.i (lock_inv l' l.r l.gr v));
         b
       }
     };
 
+  drop_ (loc l0);
   if b {
     fold (lock_alive l #p v);
     fold (lock_acquired l)
@@ -137,26 +165,35 @@ fn release (#v:slprop) (#p:perm) (l:lock)
 {
   unfold (lock_alive l #p v);
   unfold (lock_acquired l);
+  with l'. assert in_same_process l';
+  with inst. assert is_send_tag v inst;
 
   later_credit_buy 1;
   with_invariants (CInv.iname_of l.i)
     returns _:unit
-    ensures later (cinv_vp l.i (lock_inv l.r l.gr v)) **
+    ensures later (cinv_vp l.i (lock_inv l' l.r l.gr v)) **
+            in_same_process l' ** is_send_tag v inst **
             active l.i p {
+    unfold in_same_process l'; with l0. assert loc l0; loc_dup l0; fold in_same_process l';
     later_elim _;
     unpack_cinv_vp l.i;
-    unfold (lock_inv l.r l.gr v);
-    unfold (lock_inv_aux l.r l.gr v);
+    unfold (lock_inv l' l.r l.gr v);
+    is_sync_elim_on (lock_inv_aux l' l.r l.gr v) #_;
+    unfold (lock_inv_aux l' l.r l.gr v);
     GR.pts_to_injective_eq l.gr;
     GR.gather l.gr;
     with i. assert (pts_to l.gr i);
-    rewrite (if (i = 0ul) then v else emp) as emp;
-    write_atomic_box l.r 0ul;
+    rewrite on (process_of l') (if (i = 0ul) then v else emp) as on (process_of l') emp;
+    placeless_emp (process_of l') l0; on_elim emp;
     GR.(l.gr := 0ul);
-    fold (lock_inv_aux l.r l.gr v);
-    fold (lock_inv l.r l.gr v);
+    write_atomic_box l.r 0ul;
+    unsafe_attest_released v #inst #l0;
+    fold (lock_inv_aux l' l.r l.gr v);
+    is_sync_intro_on (lock_inv_aux l' l.r l.gr v) _;
+    fold (lock_inv l' l.r l.gr v);
     pack_cinv_vp l.i;
-    later_intro (cinv_vp l.i (lock_inv l.r l.gr v));
+    later_intro (cinv_vp l.i (lock_inv l' l.r l.gr v));
+    drop_ (loc l0);
   };
 
   fold (lock_alive l #p v)
@@ -170,8 +207,12 @@ fn share (#v:slprop) (#p:perm) (l:lock)
   ensures lock_alive l #(p /. 2.0R) v ** lock_alive l #(p /. 2.0R) v
 {
   unfold (lock_alive l #p v);
+  with l'. assert in_same_process l';
+  with inst. assert is_send_tag v inst;
   CInv.share l.i;
-  dup_inv (CInv.iname_of l.i) (cinv_vp l.i (lock_inv l.r l.gr v));  // make this arg implicit
+  dup (in_same_process l') ();
+  fold is_send_tag v inst;
+  dup_inv (CInv.iname_of l.i) (cinv_vp l.i (lock_inv l' l.r l.gr v));  // make this arg implicit
   fold (lock_alive l #(p /. 2.0R) v);
   fold (lock_alive l #(p /. 2.0R) v)
 } 
@@ -184,10 +225,10 @@ fn gather (#v:slprop) (#p1 #p2 :perm) (l:lock)
   ensures lock_alive l #(p1 +. p2) v
 {
   unfold (lock_alive l #p1 v);
+  drop_ (in_same_process _ ** is_send_tag v _ ** inv (iname_of l.i) _);
   unfold (lock_alive l #p2 v);
   CInv.gather #p1 #p2 l.i;
   fold (lock_alive l #(p1 +. p2) v);
-  drop_ (inv _ _)
 } 
 
 
@@ -196,16 +237,20 @@ fn free (#v:slprop) (l:lock)
   requires lock_acquired l
 {
   unfold (lock_alive l #1.0R v);
+  with l'. assert in_same_process l';
+  with inst. assert is_send_tag v inst;
   unfold (lock_acquired l);
   later_credit_buy 1;
   cancel l.i;
-  unfold (lock_inv l.r l.gr v);
-  unfold (lock_inv_aux l.r l.gr v);
+  unfold (lock_inv l' l.r l.gr v);
+  is_sync_elim_on (lock_inv_aux l' l.r l.gr v) #_;
+  unfold (lock_inv_aux l' l.r l.gr v); with i. _;
   B.free l.r;
   GR.gather l.gr;
   GR.free l.gr;
-  with i. assert (if (i = 0ul) then v else emp); // awkward
-  rewrite (if (i = 0ul) then v else emp) as emp;
+  rewrite on (process_of l') (if (i = 0ul) then v else emp) as on (process_of l') emp;
+  drop_ (on (process_of l') emp);
+  drop_ (in_same_process l' ** is_send_tag v inst);
   ()
 }
 
@@ -217,76 +262,18 @@ fn lock_alive_inj
   requires lock_alive l #p1 v1 ** lock_alive l #p2 v2
   ensures  lock_alive l #p1 v1 ** lock_alive l #p2 v1
 {
-  unfold (lock_alive l #p1 v1);
   unfold (lock_alive l #p2 v2);
-  dup_inv (CInv.iname_of l.i) (CInv.cinv_vp l.i (lock_inv l.r l.gr v1));
+  drop_ (inv _ _);
+  drop_ (is_send_tag v2 _);
+  drop_ (in_same_process _);
+  unfold (lock_alive l #p1 v1);
+  with inst. assert is_send_tag v1 inst;
+  with l1. assert in_same_process l1;
+  dup_inv (CInv.iname_of l.i) (CInv.cinv_vp l.i (lock_inv _ l.r l.gr v1));
+  dup (is_send_tag v1 inst) ();
+  dup (in_same_process l1) ();
   fold (lock_alive l #p1 v1);
   fold (lock_alive l #p2 v1);
-  drop_ (inv _ _);
   // TODO: we could also prove from, but that requires a significant amount of congruence lemmas about equiv
   // invariant_name_identifies_invariant (CInv.iname_of l.i) (CInv.iname_of l.i);
 }
-
-
-let iname_of l = CInv.iname_of l.i
-let iname_v_of l v = cinv_vp l.i (lock_inv l.r l.gr v)
-let lock_active #p l = active l.i p
-
-
-ghost
-fn share_lock_active (#p:perm) (l:lock)
-  requires lock_active #p l
-  ensures lock_active #(p /. 2.0R) l ** lock_active #(p /. 2.0R) l
-{
-  unfold (lock_active #p l);
-  CInv.share l.i;
-  fold (lock_active #(p /. 2.0R) l);
-  fold (lock_active #(p /. 2.0R) l)
-}
-
-
-
-ghost
-fn gather_lock_active (#p1 #p2:perm) (l:lock)
-  requires lock_active #p1 l ** lock_active #p2 l
-  ensures lock_active #(p1 +. p2) l
-{
-  unfold (lock_active #p1 l);
-  unfold (lock_active #p2 l);
-  CInv.gather #p1 #p2 l.i;
-  fold (lock_active #(p1 +. p2) l)
-}
-
-
-
-ghost
-fn elim_inv_and_active_into_alive (l:lock) (v:slprop) (#p:perm)
-  ensures (inv (iname_of l) (iname_v_of l v) ** lock_active #p l) @==> lock_alive l #p v
-{
-  intro (inv (iname_of l) (iname_v_of l v) ** lock_active #p l @==> lock_alive l #p v) fn _
-  {
-    rewrite each
-      iname_of l as CInv.iname_of l.i,
-      iname_v_of l v as cinv_vp l.i (lock_inv l.r l.gr v);
-    unfold (lock_active #p l);
-    fold (lock_alive l #p v)
-  };
-}
-
-
-
-ghost
-fn elim_alive_into_inv_and_active (l:lock) (v:slprop) (#p:perm)
-  requires emp
-  ensures lock_alive l #p v @==> (inv (iname_of l) (iname_v_of l v) ** lock_active #p l)
-{
-  intro (lock_alive l #p v @==> inv (iname_of l) (iname_v_of l v) ** lock_active #p l) fn _
-  {
-    unfold (lock_alive l #p v);
-    fold (lock_active #p l);
-    rewrite each
-      CInv.iname_of l.i as iname_of l,
-      cinv_vp l.i (lock_inv l.r l.gr v) as iname_v_of l v
-  };
-}
-
