lib/pulse/lib/Pulse.Lib.GhostReference.fsti
@@ -46,6 +46,9 @@ instance has_pts_to_ref (a:Type u#a) : has_pts_to (ref a) a = {
   pts_to = (fun r #f v -> pts_to r #f v);
 }
 
+instance val pts_to_placeless (#a:Type u#a) (r:ref a) (p:perm) (n:a) :
+  placeless (pts_to r #p n)
+
 val pts_to_timeless (#a:Type u#a) (r:ref a) (p:perm) (n:a)
   : Lemma (timeless (pts_to r #p n)) [SMTPat (timeless (pts_to r #p n))]
 
