lib/pulse/lib/Pulse.Lib.SendSync.fst
@@ -1,0 +1,307 @@
+module Pulse.Lib.SendSync
+open Pulse.Lib.Core
+open Pulse.Class.Duplicable
+open Pulse.Main
+#lang-pulse
+
+ghost fn dup_in_same_process p () : duplicable_f (in_same_process p) = {
+  unfold in_same_process p;
+  loc_dup _;
+  fold in_same_process p;
+  fold in_same_process p;
+}
+
+instance duplicable_in_same_process p : duplicable (in_same_process p) =
+  { dup_f = dup_in_same_process p }
+
+let can_see_writes_from (other_loc: loc_id) : slprop =
+  in_same_process other_loc **
+    emp // extra assumptions
+
+ghost fn can_see_writes_from_prop other_loc
+  preserves can_see_writes_from other_loc
+  ensures in_same_process other_loc
+{
+  unfold can_see_writes_from other_loc;
+  dup (in_same_process other_loc) ();
+  fold can_see_writes_from other_loc;
+}
+
+ghost fn writes_visible_in_prop other_loc
+  preserves writes_visible_in other_loc
+  ensures in_same_process other_loc
+{
+  unfold writes_visible_in other_loc;
+  with l. assert loc l; loc_dup l;
+  ghost_impersonate other_loc
+    (on other_loc (can_see_writes_from l))
+    (on other_loc (can_see_writes_from l) ** pure (process_of other_loc == process_of l))
+    fn _ {
+      on_elim (can_see_writes_from l);
+      can_see_writes_from_prop l;
+      on_intro (can_see_writes_from l);
+      unfold in_same_process l;
+      loc_gather other_loc #_;
+    };
+  fold in_same_process other_loc;
+  fold writes_visible_in other_loc;
+}
+
+
+[@@deprecated "UNSAFE"]
+ghost fn unsafe_attest_can_see_writes_from (other_loc: loc_id)
+    pre post (k: unit -> stt_ghost unit emp_inames (can_see_writes_from other_loc ** pre)
+      (fun _ -> can_see_writes_from other_loc ** post))
+  preserves in_same_process other_loc
+  requires pre
+  ensures post
+{
+  dup (in_same_process other_loc) ();
+  fold can_see_writes_from other_loc;
+  k ();
+  drop_ (can_see_writes_from other_loc);
+}
+
+[@@deprecated "UNSAFE"]
+ghost fn unsafe_attest_writes_visible_in (other_loc: loc_id)
+    pre post (k: unit -> stt_ghost unit emp_inames (writes_visible_in other_loc ** pre)
+      (fun _ -> writes_visible_in other_loc ** post))
+  preserves in_same_process other_loc
+  requires pre
+  ensures post
+{
+  unfold in_same_process other_loc;
+  with l. assert loc l;
+  on_intro pre;
+  ghost_impersonate other_loc (on l pre) (on l post) fn _ {
+    loc_dup other_loc;
+    fold in_same_process l;
+    unsafe_attest_can_see_writes_from l (loc other_loc ** on l pre) (loc other_loc ** on l post) fn _ {
+      on_intro (can_see_writes_from l);
+      ghost_impersonate l
+          (on other_loc (can_see_writes_from l) ** on l pre)
+          (on other_loc (can_see_writes_from l) ** on l post)
+          fn _ {
+        loc_dup l;
+        fold writes_visible_in other_loc;
+        on_elim pre;
+        k ();
+        on_intro post;
+        unfold writes_visible_in other_loc;
+        loc_gather l #_;
+      };
+      on_elim (can_see_writes_from l);
+    };
+    drop_ (in_same_process l);
+  };
+  on_elim post;
+  fold in_same_process other_loc;
+}
+
+ghost fn is_send_acq (p: slprop) {| inst: is_send p |} (other_loc: loc_id)
+  preserves can_see_writes_from other_loc
+  requires on other_loc p
+  ensures p
+{
+  inst other_loc;
+}
+
+ghost fn is_send_rel (p: slprop) {| is_send p |} (other_loc: loc_id)
+  preserves writes_visible_in other_loc
+  requires p
+  ensures on other_loc p
+{
+  unfold writes_visible_in;
+  with l. assert loc l;
+  on_intro p;
+  ghost_impersonate other_loc
+    (on other_loc (can_see_writes_from l) ** on l p)
+    (on other_loc (can_see_writes_from l) ** on other_loc p)
+    fn _ {
+      on_elim (can_see_writes_from l);
+      is_send_acq p l;
+      on_intro p;
+      on_intro (can_see_writes_from l);
+    };
+  fold writes_visible_in other_loc;
+}
+
+[@@deprecated "UNSAFE"]
+ghost fn unsafe_attest_released (p: slprop) {| is_send p |} (#l:loc_id)
+  preserves loc l
+  requires p
+  ensures on (process_of l) p
+{
+  loc_dup l;
+  fold in_same_process (process_of l);
+  unsafe_attest_writes_visible_in (process_of l) p (on (process_of l) p)
+    fn _ { is_send_rel p (process_of l) };
+  unfold in_same_process (process_of l);
+  loc_gather l #_;
+}
+
+[@@deprecated "UNSAFE"]
+ghost fn unsafe_attest_acquired (p: slprop) {| is_send p |} (#l:loc_id)
+  preserves loc l
+  requires on (process_of l) p
+  ensures p
+{
+  loc_dup l;
+  fold in_same_process (process_of l);
+  unsafe_attest_can_see_writes_from (process_of l) (on (process_of l) p) p
+    fn _ { is_send_acq p (process_of l) };
+  unfold in_same_process (process_of l);
+  loc_gather l #_;
+}
+
+ghost fn on_star_elim #l (p q: slprop)
+  requires on l (p ** q)
+  ensures on l p
+  ensures on l q
+{
+  ghost_impersonate l (on l (p ** q)) (on l p ** on l q) fn _ {
+    on_elim (p ** q);
+    on_intro p;
+    on_intro q;
+  }
+}
+
+ghost fn on_star_intro #l (p q: slprop)
+  requires on l p
+  requires on l q
+  ensures on l (p ** q)
+{
+  ghost_impersonate l (on l p ** on l q) (on l (p ** q)) fn _ {
+    on_elim p;
+    on_elim q;
+    on_intro (p ** q);
+  }
+}
+
+ghost fn on_exists_elim u#a #l (#a: Type u#a) (p: a -> slprop)
+  requires on l (exists* x. p x)
+  ensures exists* x. on l (p x)
+{
+  ghost_impersonate l (on l (exists* x. p x)) (exists* x. on l (p x)) fn _ {
+    on_elim (exists* x. p x);
+    on_intro (p _);
+  }
+}
+
+ghost fn is_send_placeless p {| inst: placeless p |} : is_send p = l {
+  loc_get (); with l0. assert loc l0;
+  inst l l0;
+  on_elim p;
+  drop_ (loc l0);
+}
+
+ghost fn is_send_star p q {| is_send p, is_send q |} : is_send (p ** q) = l {
+  on_star_elim p q;
+  is_send_acq p l;
+  is_send_acq q l;
+}
+
+ghost fn is_send_exists' u#a (#a: Type u#a) (p: a->slprop) {| ((x:a) -> is_send (p x)) |} :
+    is_send (exists* x. p x) = l {
+  on_exists_elim p;
+  with x. assert on l (p x);
+  is_send_acq (p x) l;
+}
+let is_send_exists p = is_send_exists' p
+
+ghost fn is_sync_elim p {| inst: is_sync p |} #l l'
+  requires on l p
+  requires pure (process_of l == process_of l')
+  ensures on l' p
+{
+  inst l l'
+}
+
+ghost fn is_sync_elim_on p {| is_sync p |} #l
+  preserves in_same_process l
+  requires on l p
+  ensures p
+{
+  unfold in_same_process l;
+  with l0. assert loc l0;
+  is_sync_elim p l0;
+  on_elim p;
+  fold in_same_process l;
+}
+
+ghost fn is_sync_intro_on p {| is_sync p |} l
+  preserves in_same_process l
+  requires p
+  ensures on l p
+{
+  unfold in_same_process l;
+  with l0. assert loc l0;
+  on_intro p;
+  is_sync_elim p l;
+  fold in_same_process l;
+}
+
+ghost fn is_sync_placeless p {| inst: placeless p |} : is_sync p = l l' {
+  inst l l'
+}
+
+ghost fn is_sync_in_same_process p : is_sync (in_same_process p) = l l' {
+  ghost_impersonate l
+    (on l (in_same_process p))
+    (on l' (in_same_process p))
+    fn _ {
+      on_elim (in_same_process p);
+      unfold in_same_process p;
+      loc_gather l #_;
+      ghost_impersonate l' emp (on l' (in_same_process p)) fn _ {
+        loc_dup l';
+        fold in_same_process p;
+        on_intro (in_same_process p);
+      }
+    }
+}
+
+ghost fn is_send_of_is_sync p {| is_sync p |} : is_send p = l {
+  can_see_writes_from_prop l;
+  unfold in_same_process l; with l0. assert loc l0;
+  is_sync_elim p l0;
+  on_elim p;
+  drop_ (loc l0);
+}
+
+ghost fn is_sync_star p q {| is_sync p, is_sync q |} : is_sync (p ** q) = l l' {
+  on_star_elim p q;
+  is_sync_elim p l';
+  is_sync_elim q l';
+  on_star_intro p q;
+}
+
+ghost fn is_sync_exists' u#a (#a: Type u#a) (p: a->slprop) {| ((x:a) -> is_sync (p x)) |} :
+    is_sync (exists* x. p x) = l l' {
+  ghost_impersonate l (on l (exists* x. p x)) (on l' (exists* x. p x)) fn _ {
+    on_elim (exists* x. p x);
+    with x. assert p x;
+    on_intro (p x);
+    is_sync_elim (p x) l';
+    ghost_impersonate l' (on l' (p x)) (on l' (exists* x. p x)) fn _ {
+      on_elim (p x);
+      on_intro (exists* x. p x)
+    };
+  }
+}
+let is_sync_exists = is_sync_exists'
+
+
+inline_for_extraction noextract fn fork'
+  (pre:slprop) {| is_send pre |}
+  (f: (unit -> stt unit pre (fun _ -> emp)))
+  requires pre
+{
+  loc_get (); with l. assert loc l;
+  unsafe_attest_released pre #_ #l;
+  fork (on (process_of l) pre) #_ #l fn l' {
+    unsafe_attest_acquired pre #_ #l';
+    drop_ (loc l');
+    f ();
+  };
+}
