lib/pulse/lib/Pulse.Lib.SendSync.fsti
@@ -1,0 +1,101 @@
+module Pulse.Lib.SendSync
+open Pulse.Lib.Core
+open Pulse.Class.Duplicable
+open Pulse.Main
+#lang-pulse
+
+let in_same_process p = exists* l. loc l ** pure (process_of l == process_of p)
+instance val duplicable_in_same_process p : duplicable (in_same_process p)
+
+val can_see_writes_from (other_loc: loc_id) : slprop
+let writes_visible_in (other_loc: loc_id) =
+  exists* l. loc l ** on other_loc (can_see_writes_from l)
+
+ghost fn can_see_writes_from_prop other_loc
+  preserves can_see_writes_from other_loc
+  ensures in_same_process other_loc
+
+ghost fn writes_visible_in_prop other_loc
+  preserves writes_visible_in other_loc
+  ensures in_same_process other_loc
+
+[@@deprecated "UNSAFE"]
+ghost fn unsafe_attest_can_see_writes_from (other_loc: loc_id)
+    pre post (k: unit -> stt_ghost unit emp_inames (can_see_writes_from other_loc ** pre)
+      (fun _ -> can_see_writes_from other_loc ** post))
+  preserves in_same_process other_loc
+  requires pre
+  ensures post
+
+[@@deprecated "UNSAFE"]
+ghost fn unsafe_attest_writes_visible_in (other_loc: loc_id)
+    pre post (k: unit -> stt_ghost unit emp_inames (writes_visible_in other_loc ** pre)
+      (fun _ -> writes_visible_in other_loc ** post))
+  preserves in_same_process other_loc
+  requires pre
+  ensures post
+
+[@@Tactics.Typeclasses.tcclass; erasable]
+type is_send (p: slprop) =
+  other_loc: loc_id ->
+    stt_ghost unit emp_inames
+      (can_see_writes_from other_loc ** on other_loc p)
+      (fun _ -> can_see_writes_from other_loc ** p)
+
+ghost fn is_send_acq (p: slprop) {| is_send p |} (other_loc: loc_id)
+  preserves can_see_writes_from other_loc
+  requires on other_loc p
+  ensures p
+
+ghost fn is_send_rel (p: slprop) {| is_send p |} (other_loc: loc_id)
+  preserves writes_visible_in other_loc
+  requires p
+  ensures on other_loc p
+
+[@@deprecated "UNSAFE"]
+ghost fn unsafe_attest_released (p: slprop) {| is_send p |} (#l:loc_id)
+  preserves loc l
+  requires p
+  ensures on (process_of l) p
+
+[@@deprecated "UNSAFE"]
+ghost fn unsafe_attest_acquired (p: slprop) {| is_send p |} (#l:loc_id)
+  preserves loc l
+  requires on (process_of l) p
+  ensures p
+
+instance val is_send_placeless p {| placeless p |} : is_send p
+instance val is_send_star p q {| is_send p, is_send q |} : is_send (p ** q)
+instance val is_send_exists #a (p: a->slprop) {| ((x:a) -> is_send (p x)) |} : is_send (exists* x. p x)
+
+[@@Tactics.Typeclasses.tcclass; erasable]
+type is_sync (p: slprop) =
+  l:loc_id -> l':loc_id { process_of l == process_of l' } ->
+    stt_ghost unit emp_inames (on l p) (fun _ -> on l' p)
+
+ghost fn is_sync_elim p {| inst: is_sync p |} #l l'
+  requires on l p
+  requires pure (process_of l == process_of l')
+  ensures on l' p
+
+ghost fn is_sync_elim_on p {| is_sync p |} #l
+  preserves in_same_process l
+  requires on l p
+  ensures p
+
+ghost fn is_sync_intro_on p {| is_sync p |} l
+  preserves in_same_process l
+  requires p
+  ensures on l p
+
+instance val is_sync_placeless p {| inst: placeless p |} : is_sync p
+instance val is_sync_in_same_process p : is_sync (in_same_process p)
+instance val is_send_of_is_sync p {| is_sync p |} : is_send p
+instance val is_sync_star p q {| is_sync p, is_sync q |} : is_sync (p ** q)
+instance val is_sync_exists #a (p: a->slprop) {| ((x:a) -> is_sync (p x)) |} :
+  is_sync (exists* x. p x)
+
+inline_for_extraction noextract fn fork'
+  (pre:slprop) {| is_send pre |}
+  (f: (unit -> stt unit pre (fun _ -> emp)))
+  requires pre
